$$
\begin{align*}
c^2 = a^2 + b^2 - 2abcos\gamma\\
\\
cos(x+y) = cosxcosy - sinxsiny \\

sinx = a_0 + a_1x+a_2x^2+a_3x^3+\ldots\\
sinx|_{x=0} = a_0=0\\
(sinx)' = cosx = a_1 + 2a_2x + 3a_3x^2 + \ldots, a_1 = cosx|_{x=0} = 1\\
(cosx)'=-sinx=2a_2 + 3 *2 * a_3x + \ldots, -sinx|_{x=0} = 2a_2 = 0, a_2 = 0\\
(-sinx)'=-cosx = 3 * 2 * 1 * a_3 + 4 * 3 * 2 * a_4 * x + 5 * 4 * 3 * x^2 + \ldots, -cosx|_{x=0} = 3!a_3=-1, a_3 = -\frac{1}{3!}\\
sinx = x - \frac{1}{3!}x^3 + \frac{1}{5!}x^5 - \frac{1}{7!}x^7 + \ldots\\
cosx = 1 -\frac{1}{2!}x^2 + \frac{1}{4!}x^4 - \frac{1}{6!}x^6 + \ldots\\
e^x=1 + x + \frac{1}{2!}x^2 + \frac{1}{3!}x^3 + \frac{1}{4!}x^4 + \frac{1}{5!}x^5 + \frac{1}{6!}x^6 +\frac{1}{7!}x^7 + \ldots\\
e^{ix} = 1 + ix - \frac{1}{2!}x^2 - \frac{1}{3!}ix^3 + \frac{1}{4!}x^4 - \frac{1}{5!}ix^5 - \frac{1}{6!}x^6 -\frac{1}{7!}ix^7 + \ldots\\
=(1 -\frac{1}{2!}x^2 + \frac{1}{4!}x^4 - \frac{1}{6!}x^6 + \ldots) + i( x - \frac{1}{3!}x^3 + \frac{1}{5!}x^5 - \frac{1}{7!}x^7 + \ldots)\\
=cosx + isinx\\
e^{ix} = cosx + isinx\\
e^{i(x + y)} = cos(x + y) + isin(x + y)\qquad(1)\\
e^{i(x + y)} = e^{ix}*e^{iy} = [cosx + isinx][cosy + isiny] = cosxcosy - sinxsiny + i(cosxsiny + sinxcosy)\qquad(2)\\
(1)(2):\\
cos(x + y) = cosxcosy - sinxsiny\\
sin(x + y) = sinxcosy + cosxsiny\\







\end{align*}
$$

