$$
\begin{align*}
a^x = ?\\
a^0=1\\
a^\epsilon = 1 + \epsilon'\\
K\epsilon = \epsilon'\\
a^\epsilon = 1 + K\epsilon\\
a^{n\epsilon}=(1+K\epsilon)^n=1+\binom{n}{1}K\epsilon+\binom{n}{2}(K\epsilon)^2+\binom{n}{3}(K\epsilon)^3+\ldots\\
n\rightarrow\infin, \epsilon\rightarrow o, n\epsilon=x,\epsilon=\frac{x}{n}代入上式得:\\
a^x=1+\binom{n}{1}Kx+\binom{n}{2}(Kx)^2+\binom{n}{3}(Kx)^3+\ldots\\
设K=1,则a^x=1+\binom{n}{1}x+\binom{n}{2}(x)^2+\binom{n}{3}(x)^3+\ldots\\
当x=1,n\rightarrow\infin时,a=e=2.718\ldots\\
也即:e^x=1+\binom{n}{1}x+\binom{n}{2}(x)^2+\binom{n}{3}(x)^3+\ldots\\
\\
\\
\ln(1+x)=\ln(1+\epsilon)^n\\
知，此时相当于K=1的情形，即a^{n\epsilon}=(1+K\epsilon)^n中，K=1, 则a=e\\
于是\ln(1+\epsilon)^n=\ln e^{n\epsilon}=n\epsilon\\
于是\ln (1+x)=n\epsilon，解

\end{align*}
$$

